Original_Dinitz_Refine.thy
@@ -10,108 +10,11 @@ text \<open>This theory takes the abstract definition of the Original Dinitz alg
       executable, primitives such as set operations.\<close>
 
 text \<open>For several refinement proofs in this theory, we need an additional pattern for refine_dref_type\<close>
-lemma RELATESI_in_spec(*[refine_dref_pattern]*):
+lemma RELATESI_in_spec:
   "RELATES R \<Longrightarrow> S \<le> (spec x. (x, y) \<in> R) \<Longrightarrow> S \<le> (spec x. (x, y) \<in> R)" .
 
 subsection \<open>Restructuring\<close>
-context NFlow
-begin
-definition dinitzPhaseRestructured :: "(_ flow \<times> bool) nres" where
-  "dinitzPhaseRestructured \<equiv> do {
-    stl \<leftarrow> spec c'. Dual_Shortest_Path_Union c' cf s t;
-    (f', _, _, changed) \<leftarrow> WHILE\<^sub>T
-      (\<lambda>(_, _, brk, _). \<not> brk)
-      (\<lambda>(f', stl', _, changed). do {
-        p_opt \<leftarrow> select p. Graph.isPath stl' s p t;
-        case p_opt of
-          None \<Rightarrow> return (f', stl', True, changed)
-        | Some p \<Rightarrow> do {
-            stl'' \<leftarrow> return (Graph.subtract_path stl' p);
-            stl'' \<leftarrow> spec c'. Dual_Path_Union c' stl'' s t;
-            let f' = NFlow.augment c f' (NPreflow.augmentingFlow c f' p);
-            return (f', stl'', False, True)
-          }})
-      (f, stl, False, False);
-    return (f', changed)}"
-
-definition dinitzPhaseRestructuredInvar :: "(_ flow \<times> _ graph \<times> bool \<times> bool) \<Rightarrow> bool" where
-  "dinitzPhaseRestructuredInvar \<equiv> \<lambda>(f', stl, brk, changed).
-    NFlow c s t f'
-    \<and> Bounded_Dual_Shortest_Path_Union stl (cf_of f') s t (cf.min_dist s t)
-    \<and> (Graph.connected (cf_of f') s t \<longrightarrow> cf.min_dist s t \<le> Graph.min_dist (cf_of f') s t)
-    \<and> (brk \<longrightarrow> \<not> Graph.connected stl s t)
-    \<and> (val \<le> Flow.val c s f')
-    \<and> (changed \<longleftrightarrow> f' \<noteq> f)
-    \<and> (changed \<longrightarrow> cf.connected s t)" (* \<and> (changed \<and> brk \<longrightarrow> cf.connected s t)" *)
-
-(* TODO can this be simplified to just changed \<longleftrightarrow> val < val'? *)
-lemma dinitzPhaseRestructuredInvar_alt:
-  "dinitzPhaseRestructuredInvar = (\<lambda>(f', stl, brk, changed).
-    dinitzPhaseInvar (f', stl)
-    \<and> (brk \<longrightarrow> \<not> Graph.connected stl s t)
-    \<and> (val \<le> Flow.val c s f')
-    \<and> (changed \<longleftrightarrow> f' \<noteq> f)
-    \<and> (changed \<longrightarrow> cf.connected s t))" (* TODO does this work? *)
-  unfolding dinitzPhaseInvar_def dinitzPhaseRestructuredInvar_def by simp
-
-(* TODO comment about val needed for changed inequality *)
-
-lemma dinitzPhaseRestructured_step:
-  fixes f' stl stl' changed
-  assumes PATH: "Graph.isPath stl s p t"
-      and CLEANED: "Dual_Path_Union stl' (Graph.subtract_path stl p) s t"
-      and INVAR: "dinitzPhaseRestructuredInvar (f', stl, False, changed)"
-  defines "aug_f' \<equiv> NFlow.augment c f' (NPreflow.augmentingFlow c f' p)"
-    shows "dinitzPhaseRestructuredInvar (aug_f', stl', False, True) \<and> Graph.E stl' \<subset> Graph.E stl \<and> finite (Graph.E stl)"
-proof -
-  have "Flow.val c s f' < Flow.val c s aug_f'"
-  proof -
-    from INVAR interpret f': NFlow c s t f' unfolding dinitzPhaseRestructuredInvar_def by blast
-    from INVAR PATH interpret stu: Dual_Shortest_Path_Union stl "cf_of f'" s t
-      unfolding dinitzPhaseRestructuredInvar_alt using dual_spu_if_invar_and_path by blast
-
-    have "Flow f'.cf s t (f'.augmentingFlow p)"
-      apply (intro f'.augFlow_resFlow)
-      unfolding f'.isAugmentingPath_def
-      using PATH f'.cf.isShortestPath_alt stu.shortest_path_transfer by blast
-    moreover have "0 < Flow.val f'.cf s (f'.augmentingFlow p)"
-      by (simp add: Graph.shortestPath_is_path Graph.shortestPath_is_simple PATH f'.augFlow_val f'.isAugmentingPath_def f'.resCap_gzero_aux stu.shortest_path_transfer)
-    ultimately show ?thesis unfolding aug_f'_def using f'.augment_flow_value by simp
-  qed
-  moreover have "stl' = Graph.cleaning (Graph.subtract_path stl p) s t"
-    using CLEANED Dual_Path_Union_iff_cleaning by blast
-  moreover note PATH INVAR
-  ultimately show ?thesis unfolding dinitzPhaseRestructuredInvar_alt aug_f'_def
-    using dinitzPhase_step (* TODO prettify *)
-    apply auto
-    using Graph.connected_def Dual_Shortest_Path_Union.st_connected_iff dual_spu_if_invar_and_path apply metis
-    by blast+
-qed
-
-definition "dinitzPhaseRestructured_wf_rel \<equiv> inv_image
-  (less_than_bool <*lex*> finite_psubset)
-  (\<lambda>(_, stl, brk, _). (\<not>brk, Graph.E stl))"
-
-lemma dinitzPhaseRestructured_correct:
-  "dinitzPhaseRestructured \<le> SPEC (\<lambda>(f', changed). res_dist_increasing_flow f' \<and> changed = (f' \<noteq> f) \<and> (changed \<longrightarrow> cf.connected s t))"
-  unfolding dinitzPhaseRestructured_def
-  apply (refine_vcg WHILET_rule[where I=dinitzPhaseRestructuredInvar and R=dinitzPhaseRestructured_wf_rel])
-              apply (all \<open>(simp add: dinitzPhaseRestructuredInvar_def; fail)?\<close>)
-        apply (simp add: dinitzPhaseRestructured_wf_rel_def wf_lex_prod)
-       apply (simp add: dinitzPhaseRestructuredInvar_def NFlow_axioms min_st_dist_bound)
-      apply (simp add: dinitzPhaseRestructured_step)
-     apply (simp add: dinitzPhaseRestructured_step dinitzPhaseRestructured_wf_rel_def)
-    apply (simp add: dinitzPhaseRestructuredInvar_alt Graph.connected_def)
-   apply (simp add: dinitzPhaseRestructured_wf_rel_def)
-  by (fastforce simp: dinitzPhaseRestructuredInvar_alt dinitzPhase_final)
-end
-
-
-
-
-
-
-(* TODO everything in this locale is a horrible mess. FIX! *)
+(* TODO the proofs in this locale are quite messy, fix *)
 context RGraph
 begin
 definition dinitzPhaseRestructured :: "(_ graph \<times> bool) nres" where
@@ -125,8 +28,8 @@ definition dinitzPhaseRestructured :: "(_ graph \<times> bool) nres" where
           None \<Rightarrow> return (cf', stl', True, changed)
         | Some p \<Rightarrow> do {
             stl'' \<leftarrow> return (Graph.subtract_path stl' p);
-            stl'' \<leftarrow> spec c'. Dual_Path_Union c' stl'' s t;
             cf' \<leftarrow> return (Graph.subtract_skew_path cf' p);
+            stl'' \<leftarrow> spec c'. Dual_Path_Union c' stl'' s t;
             return (cf', stl'', False, True)}})
       (cf, stl, False, False);
     return (cf', changed)}"
@@ -149,7 +52,7 @@ lemma dinitzPhaseRestructuredInvar_alt:
   by clarsimp (metis RGraph.is_NFlow RGraph.this_loc_rpg RPreGraph.rg_fo_inv)
 
 lemma dual_spu_if_invar_and_path:
-  assumes INVAR: "dinitzPhaseRestructuredInvar (cf', stl, brk, changed)"(*INVAR: "f.dinitzPhaseInvar (flow_of_cf cf', stl)"*)
+  assumes INVAR: "dinitzPhaseRestructuredInvar (cf', stl, brk, changed)"
     and PATH: "Graph.isPath stl s p t"
   shows "Dual_Shortest_Path_Union stl cf' s t"
 proof -
@@ -195,13 +98,7 @@ proof (simp, intro conjI)
     "changed = (cf' \<noteq> cf)"
     "changed \<longrightarrow> cf.connected s t"
     unfolding dinitzPhaseRestructuredInvar_def by auto
-  (*thm f.cf_def
-  then interpret f': NFlow c s t "flow_of_cf cf'" +
-    old_bounded: Bounded_Dual_Shortest_Path_Union stl cf' s t "cf.min_dist s t"
-    using RGraph.is_NFlow by simp_all
-  from \<open>RGraph c s t cf'\<close> interpret rg': RGraph c s t cf' .
-  thm f'.cf_def
-  thm rg'.f.cf_def[unfolded rg'.f_def]*)
+
   then interpret rg': RGraph c s t cf' +
     old_bounded: Bounded_Dual_Shortest_Path_Union stl cf' s t "cf.min_dist s t" by simp_all
 
@@ -229,29 +126,6 @@ proof (simp, intro conjI)
   then interpret aug_rg: RGraph c s t aug_cf' by blast
   from \<open>f.val \<le> Flow.val c s (flow_of_cf cf')\<close> have "f.val \<le> rg'.f.val" unfolding rg'.f_def .
 
-(*
-  interpret tmp: Flow c s t "flow_of_cf aug_cf'"
-    using aug_rg.f.Flow_axioms aug_rg.f_def by force
-  thm aug_rg.f.Flow_axioms
-  thm aug_rg.f_def
-  term aug_rg.f.val
-  term f.val
-  thm aug_rg.f.val_def
-  show "f.val \<le> aug_rg.f.val"
-*)
-  thm NFlow.is_RGraph
-  thm f.dinitzPhase_step
-  thm NFlow.augment_alt'
-  thm NPreflow.augmentingFlow_alt
-  thm rg'.f.augment_alt'
-  thm rg'.f.augmentingFlow_alt
-  thm rg'.f_def
-  thm rg'.rg_fo_inv
-  thm NFlow.dual_spu_if_invar_and_path
-  thm rg'.f.dual_spu_if_invar_and_path
-
-(* have "Flow.val c s f' < Flow.val c s aug_f'" *)
-
   have "f.val < Flow.val c s (flow_of_cf aug_cf')"
   proof -
     have BOUND_EQ: "cf.min_dist s t = rg'.cf.min_dist s t"
@@ -277,14 +151,10 @@ proof (simp, intro conjI)
       apply (intro rg'.f.augFlow_resFlow)
       unfolding rg'.f.isAugmentingPath_def
       using PATH rg'.f.cf.isShortestPath_alt stu.shortest_path_transfer rg'.rg_fo_inv by simp
-    thm \<open>f.val \<le> Flow.val c s (flow_of_cf cf')\<close>
-    thm aug_cf'_alt
-    thm rg'.f.augFlow_val
+
     have 1: "rg'.f.isAugmentingPath p"
       by (metis Graph.isSimplePath_def PATH \<open>rg'.cf.isPath s p t\<close> old_bounded.paths_are_simple rg'.f.isAugmentingPath_def rg'.rg_is_cf)
-    thm rg'.f.augment_flow_value[OF 0]
-    thm rg'.f.augFlow_val[OF 1]
-    thm rg'.f.resCap_gzero_aux
+    
     have "rg'.f.cf.isPath s p t" by (simp add: \<open>rg'.cf.isPath s p t\<close>)
     then have "0 < Flow.val rg'.f.cf s (rg'.f.augmentingFlow p)"
       using rg'.f.augFlow_val[OF 1] rg'.f.resCap_gzero_aux by simp
@@ -293,11 +163,6 @@ proof (simp, intro conjI)
     with \<open>f.val \<le> Flow.val c s (flow_of_cf cf')\<close> show ?thesis
       unfolding rg'.f_def using aug_cf'_alt
       by (metis "0" Flow.axioms(1) NFlow.augment_flow_presv NPreflow.is_RPreGraph NPreflow_def RPreGraph.f_unique \<open>0 < Flow.val rg'.f.cf s (rg'.f.augmentingFlow p)\<close> \<open>Flow.val c s (rg'.f.augment (rg'.f.augmentingFlow p)) = rg'.f.val + Flow.val rg'.f.cf s (rg'.f.augmentingFlow p)\<close> add.commute add_strict_increasing aug_rg.is_NPreflow aug_rg.rg_fo_inv rg'.f_def rg'.is_NFlow)
-    (*have ?thesis unfolding aug_cf'_def using rg'.f.augment_flow_value oops*)
-    (*moreover have "0 < Flow.val rg'.f.cf s (rg'.f.augmentingFlow p)"
-      unfolding rg'.f.augFlow_val
-      by (simp add: Graph.shortestPath_is_path Graph.shortestPath_is_simple PATH rg'.f.augFlow_val rg'.f.isAugmentingPath_def rg'.f.resCap_gzero_aux stu.shortest_path_transfer)*)
-    (*ultimately show ?thesis unfolding aug_f'_def using f'.augment_flow_value by simp*)
   qed
   then show "f.val \<le> Flow.val c s (flow_of_cf aug_cf')" "aug_cf' \<noteq> cf" unfolding f_def by auto
   show "cf.connected s t"
@@ -342,157 +207,9 @@ lemma dinitzPhaseRestructured_correct:
   by (simp add: dinitzPhaseRestructured_final)
 end
 
-
-(*
-find_theorems "cf_of (flow_of_cf ?cf) = ?cf"
-thm rg_fo_inv
-find_theorems "(?A \<Longrightarrow> ?B) \<Longrightarrow> (?B \<Longrightarrow> ?A) \<Longrightarrow> ?A = ?B"
-thm iffI
-(* TODO can this be simplified to just changed \<longleftrightarrow> val < val'? *)
-lemma dinitzPhaseRestructuredInvar_alt:
-  "dinitzPhaseRestructuredInvar = (\<lambda>(cf', stl, brk, changed).
-    f.dinitzPhaseInvar ((flow_of_cf cf'), stl)
-    \<and> (brk \<longrightarrow> \<not> Graph.connected stl s t)
-    \<and> (Flow.val c s f \<le> Flow.val c s (flow_of_cf cf'))
-    \<and> (changed \<longleftrightarrow> cf' \<noteq> cf)
-    \<and> (changed \<longrightarrow> cf.connected s t))"
-proof (intro ext, clarsimp, intro iffI)
-  fix cf' stl brk changed
-  assume "dinitzPhaseRestructuredInvar (cf', stl, brk, changed)"
-  then have INVAR: "RGraph c s t cf'"
-    "Bounded_Dual_Shortest_Path_Union stl cf' s t (cf.min_dist s t)"
-    "Graph.connected cf' s t \<longrightarrow> cf.min_dist s t \<le> Graph.min_dist cf' s t"
-    "brk \<longrightarrow> \<not> Graph.connected stl s t"
-    "f.val \<le> Flow.val c s (flow_of_cf cf')"
-    "changed = (cf' \<noteq> cf)"
-    "changed \<longrightarrow> cf.connected s t"
-    unfolding dinitzPhaseRestructuredInvar_def by auto
-  then interpret cf': RGraph c s t cf' by blast
-  from INVAR show "f.dinitzPhaseInvar (flow_of_cf cf', stl) \<and>
-       (brk \<longrightarrow> \<not> Graph.connected stl s t) \<and> f.val \<le> Flow.val c s (flow_of_cf cf') \<and> changed = (cf' \<noteq> cf) \<and> (changed \<longrightarrow> cf.connected s t)"
-    unfolding f.dinitzPhaseInvar_def apply clarsimp
-    using cf'.is_NFlow by fastforce
-next
-  fix cf' stl brk changed
-  assume INVAR: "f.dinitzPhaseInvar (flow_of_cf cf', stl) \<and>
-       (brk \<longrightarrow> \<not> Graph.connected stl s t) \<and> f.val \<le> Flow.val c s (flow_of_cf cf') \<and> changed = (cf' \<noteq> cf) \<and> (changed \<longrightarrow> cf.connected s t)"
-  then interpret tmp: NFlow c s t "flow_of_cf cf'" unfolding f.dinitzPhaseInvar_def by blast
-  interpret tmp2: RGraph c s t tmp.cf using tmp.is_RGraph by blast
-  from INVAR show "dinitzPhaseRestructuredInvar (cf', stl, brk, changed)"
-    unfolding dinitzPhaseRestructuredInvar_def f.dinitzPhaseInvar_def apply clarsimp oops
-  apply clarsimp
-  unfolding rg_fo_inv
-  apply (intro ext)
-  apply clarsimp apply rule
-  
-  
-  
-  apply (simp add: split_paired_all)
-
-proof (intro ext, clarsimp)
-  apply rule
-  unfolding split_paired_all apply simp
-proof 
-  unfolding dinitzPhaseRestructuredInvar_def apply clarsimp
-
-(* TODO comment about val needed for changed inequality *)
-oops end end end
-lemma dinitzPhaseRestructured_step:
-  fixes f' stl stl' changed
-  assumes PATH: "Graph.isPath stl s p t"
-      and CLEANED: "Dual_Path_Union stl' (Graph.subtract_path stl p) s t"
-      and INVAR: "dinitzPhaseRestructuredInvar (f', stl, False, changed)"
-  defines "aug_f' \<equiv> NFlow.augment c f' (NPreflow.augmentingFlow c f' p)"
-    shows "dinitzPhaseRestructuredInvar (aug_f', stl', False, True) \<and> Graph.E stl' \<subset> Graph.E stl \<and> finite (Graph.E stl)"
-proof -
-  have "Flow.val c s f' < Flow.val c s aug_f'"
-  proof -
-    from INVAR interpret f': NFlow c s t f' unfolding dinitzPhaseRestructuredInvar_def by blast
-    from INVAR PATH interpret stu: Dual_Shortest_Path_Union stl "cf_of f'" s t
-      unfolding dinitzPhaseRestructuredInvar_alt using dual_spu_if_invar_and_path by blast
-
-    have "Flow f'.cf s t (f'.augmentingFlow p)"
-      apply (intro f'.augFlow_resFlow)
-      unfolding f'.isAugmentingPath_def
-      using PATH f'.cf.isShortestPath_alt stu.shortest_path_transfer by blast
-    moreover have "0 < Flow.val f'.cf s (f'.augmentingFlow p)"
-      by (simp add: Graph.shortestPath_is_path Graph.shortestPath_is_simple PATH f'.augFlow_val f'.isAugmentingPath_def f'.resCap_gzero_aux stu.shortest_path_transfer)
-    ultimately show ?thesis unfolding aug_f'_def using f'.augment_flow_value by simp
-  qed
-  moreover have "stl' = Graph.cleaning (Graph.subtract_path stl p) s t"
-    using CLEANED Dual_Path_Union_iff_cleaning by blast
-  moreover note PATH INVAR
-  ultimately show ?thesis unfolding dinitzPhaseRestructuredInvar_alt aug_f'_def
-    using dinitzPhase_step (* TODO prettify *)
-    apply auto
-    apply (meson Graph.connected_def Dual_Shortest_Path_Union.st_connected_iff dual_spu_if_invar_and_path)
-    by blast+
-qed
-
-definition "dinitzPhaseRestructured_wf_rel \<equiv> inv_image
-  (less_than_bool <*lex*> finite_psubset)
-  (\<lambda>(_, stl, brk, _). (\<not>brk, Graph.E stl))"
-
-lemma dinitzPhaseRestructured_correct:
-  "dinitzPhaseRestructured \<le> SPEC (\<lambda>(f', changed). res_dist_increasing_flow f' \<and> changed = (f' \<noteq> f) \<and> (changed \<longrightarrow> cf.connected s t))"
-  unfolding dinitzPhaseRestructured_def
-  apply (refine_vcg WHILET_rule[where I=dinitzPhaseRestructuredInvar and R=dinitzPhaseRestructured_wf_rel])
-              apply (all \<open>(simp add: dinitzPhaseRestructuredInvar_def; fail)?\<close>)
-        apply (simp add: dinitzPhaseRestructured_wf_rel_def wf_lex_prod)
-       apply (simp add: dinitzPhaseRestructuredInvar_def NFlow_axioms min_st_dist_bound)
-      apply (simp add: dinitzPhaseRestructured_step)
-     apply (simp add: dinitzPhaseRestructured_step dinitzPhaseRestructured_wf_rel_def)
-    apply (simp add: dinitzPhaseRestructuredInvar_alt Graph.connected_def)
-   apply (simp add: dinitzPhaseRestructured_wf_rel_def)
-  by (fastforce simp: dinitzPhaseRestructuredInvar_alt dinitzPhase_final)
-end
-*)
-
-
-
-
-
-
-
-
-
-
 context Network
 begin
-definition dinitzRestructured :: "_ flow nres" where
-  "dinitzRestructured \<equiv> do {
-    (f, _) \<leftarrow> WHILE\<^sub>T snd (NFlow.dinitzPhaseRestructured c s t \<circ> fst) (\<lambda>_. 0, True);
-    return f}"
 
-theorem dinitzRestructured_correct: "dinitzRestructured \<le> (spec f. isMaxFlow f)"
-  unfolding dinitzRestructured_def
-  apply (refine_vcg WHILET_rule[where I="\<lambda>(f', m). NFlow c s t f' \<and> (m \<or> isMaxFlow f')"
-          and R="inv_image (less_than_bool <*lex*> res_dist_rel) prod.swap"])
-      apply (fastforce simp: res_dist_wf)
-     apply (clarsimp_all simp: NFlowI Network_axioms zero_is_flow)
-proof -
-  fix f
-  assume "NFlow c s t f"
-  then interpret NFlow c s t f .
-  have "dinitzPhaseRestructured \<le> SPEC (\<lambda>(f', changed). res_dist_increasing_flow f' \<and> changed = (f' \<noteq> f) \<and> (changed \<longrightarrow> cf.connected s t))"
-    using dinitzPhaseRestructured_correct .
-  also have "... \<le> (spec s'. (case s' of (f', m) \<Rightarrow> NFlow c s t f' \<and> (m \<or> isMaxFlow f')) \<and> (prod.swap s', True, f) \<in> less_than_bool <*lex*> res_dist_rel)"
-  proof (clarsimp, intro conjI)
-    fix f'
-    assume "res_dist_increasing_flow f'" and CON_IF_NEQ: "(f' \<noteq> f) \<longrightarrow> cf.connected s t"
-    then show "NFlow c s t f'"
-      unfolding res_dist_increasing_flow_def by simp
-    then interpret n': NFlow c s t f' .
-    from \<open>res_dist_increasing_flow f'\<close> have DIST: "n'.cf.connected s t \<longrightarrow> cf.min_dist s t < n'.cf.min_dist s t"
-      unfolding res_dist_increasing_flow_def by simp
-    with CON_IF_NEQ show "f' = f \<or> f' \<noteq> f \<and> (f', f) \<in> res_dist_rel" unfolding res_dist_rel_def by blast
-    from CON_IF_NEQ show "f' = f \<longrightarrow> isMaxFlow f"
-      using Graph.connected_def Graph.isSimplePath_fwd n'.fofu_III_I n'.fofu_II_III n'.isAugmentingPath_def DIST by blast
-  qed
-  finally show "dinitzPhaseRestructured \<le> (spec s'. (case s' of (f', m) \<Rightarrow> NFlow c s t f' \<and> (m \<or> isMaxFlow f')) \<and> (prod.swap s', True, f) \<in> less_than_bool <*lex*> res_dist_rel)" .
-qed
-
-thm res_dist_rel_def
 (* TODO we need only one of these to be an rgraph, check which is better *)
 (*RGraph c s t cf \<and> *)
 definition "cf_dist_rel \<equiv> {(cf', cf).
@@ -516,15 +233,14 @@ proof (rule wf_subset)
     by (fastforce simp: cf_dist_rel_def greater_bounded_def)
 qed
 
-term RGraph.dinitzPhaseRestructured
-definition dinitzRestructured' :: "_ flow nres" where
-  "dinitzRestructured' \<equiv> do {
+definition dinitzRestructured :: "_ flow nres" where
+  "dinitzRestructured \<equiv> do {
     (cf, _) \<leftarrow> WHILE\<^sub>T snd (RGraph.dinitzPhaseRestructured s t \<circ> fst) (c, True);
     f \<leftarrow> return (flow_of_cf cf);
     return f}"
 
-theorem dinitzRestructured_correct': "dinitzRestructured' \<le> (spec f. isMaxFlow f)"
-  unfolding dinitzRestructured'_def
+theorem dinitzRestructured_correct: "dinitzRestructured \<le> (spec f. isMaxFlow f)"
+  unfolding dinitzRestructured_def
   apply (refine_vcg WHILET_rule[where I="\<lambda>(cf, m). RGraph c s t cf \<and> (m \<or> isMaxFlow (flow_of_cf cf))"
           and R="inv_image (less_than_bool <*lex*> cf_dist_rel) prod.swap"])
       apply (fastforce simp: cf_dist_rel_wf)
@@ -555,82 +271,9 @@ proof -
 qed
 end
 \<comment> \<open>Restructuring\<close>
-
-
-
-
-
-
 subsection \<open>Dinitz phase refinement\<close>
 
 subsubsection \<open>Abstract version with assertions\<close>
-context NFlow
-begin
-definition dinitzPhaseAssert :: "(_ flow \<times> bool) nres" where
-  "dinitzPhaseAssert \<equiv> do {
-    stl \<leftarrow> spec c'. Dual_Shortest_Path_Union c' cf s t;
-    (f', _, _, changed) \<leftarrow> WHILE\<^sub>T\<^bsup>dinitzPhaseRestructuredInvar\<^esup>
-      (\<lambda>(_, _, brk, _). \<not> brk)
-      (\<lambda>(f', stl', _, changed). do {
-        p_opt \<leftarrow> select p. Graph.isPath stl' s p t;
-        case p_opt of
-          None \<Rightarrow> return (f', stl', True, changed)
-        | Some p \<Rightarrow> do {
-            assert (Graph.isPath stl' s p t);
-            assert (Dual_Shortest_Path_Union stl' (cf_of f') s t);
-            stl'' \<leftarrow> return (Graph.subtract_path stl' p);
-            assert (Contained_Graph stl'' stl');
-            assert (Graph.E stl' \<subseteq> Graph.E stl'' \<union> set p);
-            stl'' \<leftarrow> spec c'. Dual_Path_Union c' stl'' s t;
-            let f' = NFlow.augment c f' (NPreflow.augmentingFlow c f' p);
-            return (f', stl'', False, True)
-          }})
-      (f, stl, False, False);
-    return (f', changed)}"
-
-lemma dinitzPhaseAssert_correct:
-  "dinitzPhaseAssert \<le> SPEC (\<lambda>(f', changed). res_dist_increasing_flow f' \<and> changed = (f' \<noteq> f) \<and> (changed \<longrightarrow> cf.connected s t))"
-  unfolding dinitzPhaseAssert_def
-  apply (refine_vcg WHILEIT_rule[where R=dinitzPhaseRestructured_wf_rel])
-                      apply (all \<open>(simp add: dinitzPhaseRestructuredInvar_def; fail)?\<close>)
-              apply (simp add: dinitzPhaseRestructured_wf_rel_def wf_lex_prod)
-          apply (simp add: dinitzPhaseRestructuredInvar_def NFlow_axioms min_st_dist_bound)
-         apply (fastforce simp: dinitzPhaseRestructuredInvar_alt intro: dual_spu_if_invar_and_path)
-(*
-        apply clarsimp subgoal for _ f' stl _ changed p
-  proof -
-    interpret cf': Graph "cf_of f'" .
-    assume INVAR: "dinitzPhaseRestructuredInvar (f', stl, False, changed)"
-      and PATH: "Graph.isPath stl s p t"
-      and DSPU: "Dual_Shortest_Path_Union stl (cf_of f') s t"
-
-  then show "Dual_Shortest_Path_Union stl (cf_of f') s t"
-    unfolding dinitzPhaseAssertInvar_alt using dual_spu_if_invar_and_path by blast*)
-    defer
-        apply (simp add: Graph.subtract_path_alt) using Graph.subtract_graph_untouched_edges apply (metis (no_types, lifting) Graph.isPath_alt Graph.path_induced_graph_edges Int_Un_eq(4) Int_absorb1 Int_commute Un_Diff_cancel2 cf.isPath.simps(1) set_eq_subset t_not_s)
-       apply (simp add: dinitzPhaseRestructured_step)
-      apply (simp add: dinitzPhaseRestructured_step dinitzPhaseRestructured_wf_rel_def)
-     apply (simp add: dinitzPhaseRestructuredInvar_alt Graph.connected_def)
-    apply (simp add: dinitzPhaseRestructured_wf_rel_def)
-   apply (fastforce simp: dinitzPhaseRestructuredInvar_alt dinitzPhase_final)
-proof clarsimp_all
-  fix f' stl p changed
-  interpret cf': Graph "cf_of f'" .
-  assume INVAR: "dinitzPhaseRestructuredInvar (f', stl, False, changed)"
-     and PATH: "Graph.isPath stl s p t"
-     and "Dual_Shortest_Path_Union stl (cf_of f') s t"
-  then interpret Dual_Shortest_Path_Union stl "cf_of f'" s t + f': NFlow c s t f'
-    by (auto simp: dinitzPhaseRestructuredInvar_def)
-  interpret g': Nonnegative_Graph stl
-    using f'.cf.Nonnegative_Graph_axioms sg_Nonnegative_Graph by blast
-  (* TODO replace this with a simple 'have', need some way to use sublocale relations *)
-  interpret subt_pos_cont: Pos_Contained_Graph "g'.subtract_path p" stl
-    unfolding g'.subtract_path_alt
-    using g'.path_induced_graph_pos_contained Pos_Contained_Graph.subtract_le_contained by blast
-  show "Contained_Graph (g'.subtract_path p ) stl" by intro_locales
-qed
-end
-
 context RGraph
 begin
 definition dinitzPhaseAssert :: "(_ graph \<times> bool) nres" where
@@ -670,7 +313,6 @@ lemma dinitzPhaseAssert_correct:
     apply (simp add: dinitzPhaseRestructured_wf_rel_def)
   apply (simp add: dinitzPhaseRestructured_final)
 proof clarsimp_all
-
   fix cf' stl p changed
   assume INVAR: "dinitzPhaseRestructuredInvar (cf', stl, False, changed)"
      and PATH: "Graph.isPath stl s p t"
@@ -692,60 +334,6 @@ end
 \<comment> \<open>Abstract version with assertions\<close>
 
 subsubsection \<open>Refining the assertion version\<close>
-context NFlow
-begin
-definition dinitzPhaseRefine :: "(_ flow \<times> bool) nres" where
-  "dinitzPhaseRefine \<equiv> do {
-    stl \<leftarrow> cf.buildDualLayering s t;
-    (f', _, _, changed) \<leftarrow> WHILE\<^sub>T
-      (\<lambda>(_, _, brk, _). \<not> brk)
-      (\<lambda>(f', stl', _, changed). do {
-        p_opt \<leftarrow> Graph.greedyPathFinding stl' s t;
-        case p_opt of
-          None \<Rightarrow> return (f', stl', True, changed)
-        | Some p \<Rightarrow> do {
-            stl'' \<leftarrow> Graph.subtractPathRefine stl' p;
-            stl'' \<leftarrow> cleaningRefine p stl'';
-            let f' = NFlow.augment c f' (NPreflow.augmentingFlow c f' p);
-            return (f', stl'', False, True)
-          }})
-      (f, stl, False, False);
-    return (f', changed)}"
-
-lemma dinitzPhaseRefine_refine:
-  notes [refine_dref_pattern] = RELATESI_in_spec
-  shows "dinitzPhaseRefine \<le> \<Down> Id dinitzPhaseAssert"
-  unfolding dinitzPhaseRefine_def dinitzPhaseAssert_def
-proof (refine_rcg, refine_dref_type, clarsimp_all)
-  show "cf.buildDualLayering s t \<le> (spec c'. Dual_Shortest_Path_Union c' cf s t)"
-    using cf.buildDualLayering_correct .
-
-  fix f' stl' changed
-  assume "dinitzPhaseRestructuredInvar (f', stl', False, changed)"
-  then interpret bdspu: Bounded_Dual_Shortest_Path_Union stl' "cf_of f'" s t "cf.min_dist s t"
-    unfolding dinitzPhaseRestructuredInvar_def by blast
-  show "bdspu.g'.greedyPathFinding s t \<le> (select p. bdspu.g'.isPath s p t)"
-    using bdspu.greedyPathFinding_correct .
-next
-  fix f' stl' p
-  assume "Dual_Shortest_Path_Union stl' (cf_of f') s t"
-  then interpret dspu: Dual_Shortest_Path_Union stl' "cf_of f'" s t .
-
-  assume PATH: "dspu.g'.isPath s p t"
-  then have "dspu.g'.subtractPathRefine p = return (dspu.g'.subtract_path p)"
-    using dspu.g'.isSPath_distinct dspu.paths_are_simple dspu.g'.subtractPathRefine_correct by blast
-  then show "dspu.g'.subtractPathRefine p \<le> RES {dspu.g'.subtract_path p}" by simp
-
-  fix stl''
-  assume "Contained_Graph stl'' stl'" "dspu.E' \<subseteq> Graph.E stl'' \<union> set p"
-  with PATH show "cleaningRefine p stl'' \<le> (spec c''. Dual_Path_Union c'' stl'' s t)"
-    using dspu.Finite_Graph_EI dspu.sub_Finite_Graph dspu.cleaningRefine_correct by blast
-qed
-
-lemma dinitzPhaseRefine_correct: "dinitzPhaseRefine \<le> SPEC (\<lambda>(f', changed). res_dist_increasing_flow f' \<and> changed = (f' \<noteq> f) \<and> (changed \<longrightarrow> cf.connected s t))"
-  using dinitzPhaseRefine_refine dinitzPhaseAssert_correct by simp
-end
-
 context RGraph
 begin
 definition dinitzPhaseRefine :: "(_ graph \<times> bool) nres" where
@@ -810,41 +398,6 @@ end
 subsection \<open>Dinitz outer loop refinement\<close>
 context Network
 begin
-(*
-definition dinitzRefine :: "_ flow nres" where
-  "dinitzRefine \<equiv> do {
-    (f, _) \<leftarrow> WHILE\<^sub>T snd (NFlow.dinitzPhaseRefine c s t \<circ> fst) (\<lambda>_. 0, True);
-    return f}"
-
-theorem dinitzRefine_correct: "dinitzRefine \<le> (spec f. isMaxFlow f)"
-  unfolding dinitzRefine_def
-  apply (refine_vcg WHILET_rule[where I="\<lambda>(f', m). NFlow c s t f' \<and> (m \<or> isMaxFlow f')"
-          and R="inv_image (less_than_bool <*lex*> res_dist_rel) prod.swap"])
-      apply (fastforce simp: res_dist_wf)
-     apply (clarsimp_all simp: NFlowI Network_axioms zero_is_flow)
-proof -
-  fix f
-  assume "NFlow c s t f"
-  then interpret NFlow c s t f .
-  have "dinitzPhaseRefine \<le> SPEC (\<lambda>(f', changed). res_dist_increasing_flow f' \<and> changed = (f' \<noteq> f) \<and> (changed \<longrightarrow> cf.connected s t))"
-    using dinitzPhaseRefine_correct .
-  also have "... \<le> (spec s'. (case s' of (f', m) \<Rightarrow> NFlow c s t f' \<and> (m \<or> isMaxFlow f')) \<and> (prod.swap s', True, f) \<in> less_than_bool <*lex*> res_dist_rel)"
-  proof (clarsimp, intro conjI)
-    fix f'
-    assume "res_dist_increasing_flow f'" and CON_IF_NEQ: "(f' \<noteq> f) \<longrightarrow> cf.connected s t"
-    then show "NFlow c s t f'"
-      unfolding res_dist_increasing_flow_def by simp
-    then interpret n': NFlow c s t f' .
-    from \<open>res_dist_increasing_flow f'\<close> have DIST: "n'.cf.connected s t \<longrightarrow> cf.min_dist s t < n'.cf.min_dist s t"
-      unfolding res_dist_increasing_flow_def by simp
-    with CON_IF_NEQ show "f' = f \<or> f' \<noteq> f \<and> (f', f) \<in> res_dist_rel" unfolding res_dist_rel_def by blast
-    from CON_IF_NEQ show "f' = f \<longrightarrow> isMaxFlow f"
-      using Graph.connected_def Graph.isSimplePath_fwd n'.fofu_III_I n'.fofu_II_III n'.isAugmentingPath_def DIST by blast
-  qed 
-  finally show "dinitzPhaseRefine \<le> (spec s'. (case s' of (f', m) \<Rightarrow> NFlow c s t f' \<and> (m \<or> isMaxFlow f')) \<and> (prod.swap s', True, f) \<in> less_than_bool <*lex*> res_dist_rel)" .
-qed
-*)
-
 definition dinitzRefine :: "_ flow nres" where
   "dinitzRefine \<equiv> do {
     (cf, _) \<leftarrow> WHILE\<^sub>T snd (RGraph.dinitzPhaseRefine c s t \<circ> fst) (c, True);
@@ -883,29 +436,4 @@ proof -
 qed
 end
 \<comment> \<open>Dinitz outer loop refinement\<close>
-
-(* TODO directly refine entire programm *)
-(*
-definition dinitzRefine :: "_ flow nres" where
-  "dinitzRefine \<equiv> do {
-    (f, _) \<leftarrow> WHILE\<^sub>T snd
-      (\<lambda>(f, _). do {
-        stl \<leftarrow> Graph.buildDualLayering (cf_of f) s t;
-        (f', _, _, changed) \<leftarrow> WHILE\<^sub>T
-          (\<lambda>(_, _, brk, _). \<not> brk)
-          (\<lambda>(f', stl', _, changed). do {
-            p_opt \<leftarrow> Graph.greedyPathFinding stl' s t;
-            case p_opt of
-              None \<Rightarrow> return (f', stl', True, changed)
-            | Some p \<Rightarrow> do {
-                stl'' \<leftarrow> Graph.subtractPathRefine stl' p;
-                stl'' \<leftarrow> cleaningRefine p stl'';
-                let f' = NFlow.augment c f' (NPreflow.augmentingFlow c f' p);
-                return (f', stl'', False, True)
-              }})
-          (f, stl, False, False);
-        return (f', changed)})
-      (\<lambda>_. 0, True);
-    return f}"
-*)
 end
