Graph_Restriction.thy
@@ -122,51 +122,6 @@ begin
 sublocale Splittable_Subgraph_Path_Kind_Union by intro_locales
 end
 
-(* TODO *)
-(*
-lemma Dual_Union_right_leftI:
-  assumes REGULAR_PATH_KIND: "Regular_Path_Kind isKindPath"
-    and RIGHT: "Source_Graph_Prop_Union isKindPath c' c s"
-    and LEFT: "Target_Graph_Prop_Union isKindPath c'' c' t"
-  shows "Dual_Graph_Prop_Union isKindPath c'' c s t"
-proof
-  from REGULAR_PATH_KIND interpret Regular_Path_Kind isKindPath .
-  from RIGHT interpret right: Source_Graph_Prop_Union isKindPath c' c s .
-  interpret right: Regular_Path_Kind_Union isKindPath c' c "{s}" right.V by intro_locales
-  from LEFT interpret left: Target_Graph_Prop_Union isKindPath c'' c' t .
-  interpret left: Regular_Path_Kind_Union isKindPath c'' c' right.V' "{t}" by intro_locales
-
-  thm right.ST_path_remains
-  thm left.ST_path_remains
-
-  show "\<And>e. c'' e = 0 \<or> c e = 0 \<or> c'' e = c e"
-    by (metis left.c'_sg_c_old right.c'_sg_c_old)
-
-  show "left.E' = \<Union> {set p |p. isKindPath c s p t}"
-  proof (intro pair_set_eqI)
-    fix u v
-    assume "(u, v) \<in> \<Union> {set p |p. right.isShortestPath s p t}"
-    then obtain p where SP: "(u, v) \<in> set p" "right.isShortestPath s p t" by blast
-    then have "s \<in> right.V" "t \<in> right.V" using right.distinct_nodes_in_V_if_connected right.isShortestPath_level_edge
-      by (metis right.min_dist_z empty_set ex_in_conv right.isShortestPath_min_dist_def length_0_conv)+
-    with SP have "right.g'.isShortestPath s p t" using right.ST_path_remains sorry by blast
-    with \<open>(u, v) \<in> set p\<close> \<open>s \<in> right.V\<close> show "(u, v) \<in> left.E'" using left.target_path_union
-      using Graph.isEmpty_def Graph.isPath_edgeset Graph.isShortestPath_min_dist_def right.s_in_V_if_nonempty by fastforce
-  next
-    fix u v
-    assume "(u, v) \<in> left.E'"
-    then obtain p w where "(u, v) \<in> set p" "w \<in> right.V'" "isKindPath c' w p t"
-      using left.target_path_union by blast
-    then have "right.g'.connected s w"
-      using right.obtain_connected_subgraph_ST by blast
-    then obtain p' where "isKindPath c' s p' w" using connecting by blast
-    with \<open>right.g'.isShortestPath w p t\<close> have "right.isShortestPath s (p' @ p) t"
-      using right.g'.shortestPath_is_path right.g'.isPath_append right.shortest_path_transfer by blast
-    with \<open>(u, v) \<in> set p\<close> show "(u, v) \<in> \<Union> {set p |p. right.isShortestPath s p t}" by auto
-  qed
-qed
-*)
-
 locale Path_Union = Graph_Prop_Union Graph.isPath
 sublocale Path_Union \<subseteq> Regular_Path_Kind_Union Graph.isPath by intro_locales
 
